Main.lean
@@ -3,7 +3,8 @@ import MinimalFvExample
 open Demo
 
 def main : IO Unit := do
-  let input : List Nat := [1, 2, 3, 4, 5]
-  IO.println s!"input    : {input}"
-  IO.println s!"impl xs  : {impl input}"
-  IO.println s!"spec xs  : {reverseSpec input}"
+  let input : Array Int256 :=
+    #[1, 2, 3, 4, 5].map (BitVec.ofNat 256)
+  IO.println s!"input    : {input.toList.map BitVec.toNat}"
+  IO.println s!"impl xs  : {(impl input).toList.map BitVec.toNat}"
+  IO.println s!"spec xs  : {(reverseSpec input).map BitVec.toNat}"
